fiat2/src/fiat2/TransfSound.v
@@ -1,0 +1,314 @@
+Require Import fiat2.Language fiat2.Interpret fiat2.Value fiat2.TypeSystem fiat2.TypeSound fiat2.Utils fiat2.IndexInterface.
+Require Import coqutil.Map.Interface coqutil.Word.Interface.
+Require Import List String ZArith Morphisms.
+Import ListNotations.
+
+Section WithMap.
+  Context {width: Z} {word: word.word width} {word_ok: word.ok word}.
+  Notation value := (value (width:=width)).
+  Context {tenv : map.map string type} {tenv_ok : map.ok tenv}.
+  Context {locals : map.map string value} {locals_ok : map.ok locals}.
+
+  Definition preserve_ty Gstore f :=
+    forall e t (Genv : tenv),
+      tenv_wf Gstore -> tenv_wf Genv ->
+      type_of Gstore Genv e t -> type_of Gstore Genv (f e) t.
+
+  Definition preserve_sem Gstore store f :=
+    forall e t (Genv : tenv) (env : locals),
+      tenv_wf Gstore -> tenv_wf Genv ->
+      type_of Gstore Genv e t ->
+      locals_wf Gstore store -> locals_wf Genv env ->
+      interp_expr store env (f e) = interp_expr store env e.
+
+  Definition transf_sound (f : tenv -> tenv -> command -> command) :=
+    forall (Gstore Genv : tenv) c,
+      tenv_wf Gstore -> tenv_wf Genv ->
+      well_typed Gstore Genv c ->
+      well_typed Gstore Genv (f Gstore Genv c) /\
+        forall (store env : locals),
+          locals_wf Gstore store -> locals_wf Genv env ->
+          interp_command store env (f Gstore Genv c) = interp_command store env c.
+
+  Lemma transf_sound_compose : forall f g,
+      transf_sound f -> transf_sound g ->
+      transf_sound (fun Gstore Genv => Basics.compose (f Gstore Genv) (g Gstore Genv)).
+  Proof.
+    unfold transf_sound; intros * H_f H_g; intros.
+    apply H_g in H1; auto; destruct H1.
+    apply H_f in H1; intuition idtac.
+    rewrite H4, H2; auto.
+  Qed.
+
+  Lemma transf_sound__preserve_sem : forall f,
+      transf_sound f ->
+      forall (Gstore Genv : tenv) (c : command),
+        tenv_wf Gstore -> tenv_wf Genv ->
+        well_typed Gstore Genv c ->
+        forall (store env : locals),
+          locals_wf Gstore store -> locals_wf Genv env ->
+          interp_command store env (f Gstore Genv c) = interp_command store env c.
+  Proof.
+    unfold transf_sound; intuition idtac.
+    apply H; auto.
+  Qed.
+
+  Definition expr_transf_sound (f : expr -> expr) :=
+    forall Gstore Genv e t,
+      tenv_wf Gstore -> tenv_wf Genv ->
+      type_of Gstore Genv e t ->
+      type_of Gstore Genv (f e) t /\
+        forall (store env : locals),
+          locals_wf Gstore store -> locals_wf Genv env ->
+          interp_expr store env (f e) = interp_expr store env e.
+
+  Lemma expr_transf_sound_compose : forall f g,
+      expr_transf_sound f -> expr_transf_sound g ->
+      expr_transf_sound (Basics.compose f g).
+  Proof.
+    unfold expr_transf_sound; intros * H_f H_g; intros.
+    apply H_g in H1; auto; destruct H1.
+    apply H_f in H1; intuition idtac.
+    rewrite H4, H2; auto.
+  Qed.
+
+  Definition holds_for_all_entries {A : Type} {m : map.map string A} (P : string -> A -> Prop) (G : m) :=
+    forall k v, map.get G k = Some v -> P k v.
+
+  Definition rm_from_pred (P : string -> value -> Prop) (x : string) :=
+    fun s v => s = x \/ P s v.
+
+  Inductive parameterized_wf (Gstore Genv : tenv) (P : string -> value -> Prop) : command -> Prop :=
+  | PWCSkip : parameterized_wf Gstore Genv P CSkip
+  | PWCSeq c1 c2 : parameterized_wf Gstore Genv P c1 ->
+                   parameterized_wf Gstore Genv P c2 ->
+                   parameterized_wf Gstore Genv P (CSeq c1 c2)
+  | PWCLet e t x c : type_of Gstore Genv e t ->
+                     parameterized_wf Gstore (map.put Genv x t) P c ->
+                     parameterized_wf Gstore Genv P (CLet e x c)
+  | PWCLetMut e t x c :
+    type_of Gstore Genv e t ->
+    parameterized_wf (map.put Gstore x t) Genv (rm_from_pred P x) c ->
+    parameterized_wf Gstore Genv P (CLetMut e x c)
+  | PWCAssign x t e :
+    (forall store env, holds_for_all_entries P store ->
+                       locals_wf Gstore store -> locals_wf Genv env ->
+                       P x (interp_expr store env e)) ->
+    map.get Gstore x = Some t ->
+    type_of Gstore Genv e t ->
+    parameterized_wf Gstore Genv P (CAssign x e)
+  | PWCIf e c1 c2 : type_of Gstore Genv e TBool ->
+                    parameterized_wf Gstore Genv P c1 ->
+                    parameterized_wf Gstore Genv P c2 ->
+                    parameterized_wf Gstore Genv P (CIf e c1 c2)
+  | PWCForeach e t x c : type_of Gstore Genv e (TList t) ->
+                         parameterized_wf Gstore (map.put Genv x t) P c ->
+                         parameterized_wf Gstore Genv P (CForeach e x c).
+
+  Lemma parameterized_wf__well_typed : forall Gstore Genv P c,
+      parameterized_wf Gstore Genv P c -> well_typed Gstore Genv c.
+  Proof.
+    intros. induction H.
+    all: econstructor; eauto.
+  Qed.
+
+  Lemma parameterized_wf__preserve_P : forall Gstore Genv store env P c,
+      tenv_wf Gstore -> tenv_wf Genv ->
+      parameterized_wf Gstore Genv P c ->
+      locals_wf Gstore store -> locals_wf Genv env ->
+      holds_for_all_entries P store ->
+      holds_for_all_entries P (interp_command store env c).
+  Proof.
+    intros. generalize dependent store; generalize dependent env.
+    induction H1; simpl; auto; intros.
+    1:{ apply IHparameterized_wf2; auto. eapply command_type_sound; eauto.
+        eapply parameterized_wf__well_typed; eauto. }
+    1:{ apply IHparameterized_wf; eauto with fiat2_hints. }
+    1:{ unfold holds_for_all_entries. intros. get_update_same_diff x k.
+        1:{ rewrite Properties.map.get_update_same in *. auto. }
+        1:{ rewrite Properties.map.get_update_diff in *; try congruence.
+            unfold rm_from_pred in *.
+            apply IHparameterized_wf in H6; eauto with fiat2_hints.
+            1:{ intuition auto. congruence. }
+            unfold holds_for_all_entries; intros.
+            get_put_same_diff x k0; rewrite_map_get_put_hyp. } }
+    1:{ unfold holds_for_all_entries; intros.
+        get_put_same_diff x k; rewrite_map_get_put_hyp.
+        do_injection. apply H1; auto. }
+    1:{ apply_type_sound e. invert_type_of_value. case_match; auto. }
+    1:{ apply_type_sound e. invert_type_of_value. clear H' H6.
+        generalize dependent store. induction l; simpl; auto; intros.
+        invert_Forall; apply IHl; auto.
+        2:{ apply IHparameterized_wf; eauto with fiat2_hints. }
+        eapply command_type_sound.
+        5: apply locals_wf_step. all: eauto with fiat2_hints.
+        eapply parameterized_wf__well_typed; eauto. }
+  Qed.
+
+  Section WithPv.
+    Context (Pv : value -> Prop).
+
+    Definition value_wf_with_globals globals (x : string) (v : value) :=
+      Forall (fun tbl => x <> tbl \/ Pv v) globals.
+
+    Lemma not_In__value_wf_with_globals : forall x globals (store : locals) v,
+        ~In x globals ->
+        holds_for_all_entries (value_wf_with_globals globals) store ->
+        holds_for_all_entries (value_wf_with_globals globals) (map.put store x v).
+    Proof.
+      unfold holds_for_all_entries; intros.
+      unfold value_wf_with_globals in *.
+      destruct (String.eqb k x) eqn:E; rewrite ?eqb_eq, ?eqb_neq in *; subst; rewrite_map_get_put_hyp.
+      rewrite Forall_forall; intros. left; intro contra; subst; auto.
+    Qed.
+
+    Definition iff2 {A B} (P Q : A -> B -> Prop) :=
+      forall a b, P a b <-> Q a b.
+
+    Lemma iff2_refl : forall A B (P : A -> B -> Prop),
+        iff2 P P.
+    Proof.
+      unfold iff2; intros; intuition auto.
+    Qed.
+
+    Lemma iff2_sym : forall A B (P Q : A -> B -> Prop),
+        iff2 P Q -> iff2 Q P.
+    Proof.
+      unfold iff2; intros; apply iff_sym; auto.
+    Qed.
+
+    Lemma iff2_trans : forall A B (P Q R : A -> B -> Prop),
+        iff2 P Q -> iff2 Q R -> iff2 P R.
+    Proof.
+      unfold iff2; split; intros.
+      1: apply H0, H; auto.
+      1: apply H, H0; auto.
+    Qed.
+
+    Add Parametric Relation A B : (A -> B -> Prop) iff2
+        reflexivity proved by (iff2_refl A B)
+        symmetry proved by (iff2_sym A B)
+        transitivity proved by (iff2_trans A B)
+        as iff2_rel.
+
+    Instance rm_from_pred_Proper : Proper (iff2 ==> eq ==> iff2) rm_from_pred.
+    Proof.
+      intros P Q H x x' Hx.
+      unfold iff2, rm_from_pred; intros.
+      subst; intuition auto.
+      all: right; apply H; auto.
+    Qed.
+
+    Instance holds_for_all_entries_Proper {A : Type} {m : map.map string A} : Proper (iff2 ==> eq ==> iff) (holds_for_all_entries (m:=m)).
+    Proof.
+      intros P Q H x x' Hx.
+      unfold holds_for_all_entries. split; intros.
+      all: subst; apply H, H0; auto.
+    Qed.
+
+    Lemma iff2_parameterized_wf : forall x y z P Q,
+        iff2 P Q ->
+        parameterized_wf x y P z -> parameterized_wf x y Q z.
+    Proof.
+      intros * H_iff2 H_wf. generalize dependent Q.
+      induction H_wf; intros.
+      all: econstructor; eauto.
+      1:{ apply IHH_wf. erewrite H_iff2; auto using iff2_refl. }
+      1:{ intros. apply H_iff2, H; auto.
+          rewrite H_iff2; auto. }
+    Qed.
+
+    Instance parameterized_wf_Proper : Proper (eq ==> eq ==> iff2 ==> eq ==> iff) parameterized_wf.
+    Proof.
+      intros x x' Hx y y' Hy P Q H z z' Hz.
+      split; subst; apply iff2_parameterized_wf;
+        auto using iff2_sym.
+    Qed.
+
+    Lemma rm_not_in_globals : forall x globals,
+        ~In x globals ->
+        iff2 (rm_from_pred (value_wf_with_globals globals) x) (value_wf_with_globals globals).
+    Proof.
+      unfold iff2, rm_from_pred, value_wf_with_globals; intros.
+      induction globals; intuition auto; subst.
+      rewrite Forall_forall; intros.
+      left. intro contra; subst; auto.
+    Qed.
+  End WithPv.
+
+  Section WithGlobals.
+    Context (globals : list string).
+    Context (global_types : list type) (global_types_ok : List.length globals = List.length global_types).
+
+    Definition tenv_wf_with_globals Gstore :=
+      Forall2 (fun x t => map.get Gstore x = Some t) globals global_types.
+
+    Lemma tenv_wf_with_globals_step : forall Gstore x t,
+        tenv_wf_with_globals Gstore ->
+        ~ In x globals ->
+        tenv_wf_with_globals (map.put Gstore x t).
+    Proof.
+      intros * H ?. unfold tenv_wf_with_globals in *.
+      induction H; auto. constructor.
+      2: apply IHForall2; intuition.
+      rewrite map.get_put_diff; intuition.
+      lazymatch goal with H: _ -> False |- _ => apply H end.
+      constructor; auto.
+    Qed.
+
+    Lemma not_In__tenv_wf_with_globals : forall x t Gstore,
+        ~ In x globals -> tenv_wf_with_globals Gstore -> tenv_wf_with_globals (map.put Gstore x t).
+    Proof.
+      intros * H_not_in H. unfold tenv_wf_with_globals in *.
+      induction H; auto.
+      constructor. 2: apply IHForall2; intuition.
+      rewrite map.get_put_diff; intuition.
+      apply H_not_in; subst; intuition.
+    Qed.
+  End WithGlobals.
+
+  Section WithIndex.
+    Context {consistency : Type} (consistent : consistency -> value -> value -> Prop).
+    Context {to_from_con from_to_con : consistency}.
+    Context {idx : IndexInterface.index} {idx_wf : value -> Prop} {idx_ok : ok to_from_con from_to_con idx idx_wf consistent}.
+
+    Definition expr_aug_transf_sound (f : string -> expr -> expr) : Prop :=
+      forall Gstore Genv tbl tbl_ty e t,
+        tenv_wf Gstore -> tenv_wf Genv ->
+        type_wf tbl_ty -> is_tbl_ty tbl_ty = true ->
+        tenv_wf_with_globals [tbl] [idx_ty tbl_ty] Gstore ->
+        type_of Gstore Genv e t ->
+        type_of Gstore Genv (f tbl e) t /\
+          forall store env,
+            locals_wf Gstore store -> locals_wf Genv env ->
+            holds_for_all_entries (value_wf_with_globals idx_wf [tbl]) store ->
+            interp_expr store env (f tbl e) = interp_expr store env e.
+
+    Definition aug_transf_sound (f : string -> command -> command) : Prop :=
+      forall Gstore Genv tbl t c,
+        tenv_wf Gstore -> tenv_wf Genv ->
+        type_wf t -> is_tbl_ty t = true ->
+        tenv_wf_with_globals [tbl] [idx_ty t] Gstore ->
+        well_typed Gstore Genv c ->
+        parameterized_wf Gstore Genv (value_wf_with_globals idx_wf [tbl]) c ->
+        well_typed Gstore Genv (f tbl c) /\
+          parameterized_wf Gstore Genv (value_wf_with_globals idx_wf [tbl]) (f tbl c) /\
+          forall store env,
+            locals_wf Gstore store -> locals_wf Genv env ->
+            holds_for_all_entries (value_wf_with_globals idx_wf [tbl]) store ->
+            interp_command store env (f tbl c) = interp_command store env c.
+
+    Lemma aug_transf_sound_compose : forall f g,
+        aug_transf_sound f -> aug_transf_sound g ->
+        aug_transf_sound (fun x => Basics.compose (f x) (g x)).
+    Proof.
+      unfold aug_transf_sound; intros * H_f H_g; intros.
+      eapply H_g in H4; eauto; repeat destruct_and.
+      eapply H_f in H4; eauto; intuition idtac.
+      rewrite H10; auto.
+    Qed.
+  End WithIndex.
+End WithMap.
+
+#[export] Hint Resolve transf_sound_compose : transf_hints.
+#[export] Hint Resolve aug_transf_sound_compose : transf_hints.
