fiat2/src/fiat2/TransfUtils.v
@@ -1,0 +1,637 @@
+Require Import fiat2.Language fiat2.Interpret fiat2.Value fiat2.TypeSystem fiat2.TypeSound fiat2.Utils fiat2.TransfSound fiat2.IndexInterface.
+Require Import coqutil.Map.Interface coqutil.Word.Interface.
+Require Import List String ZArith Permutation Morphisms.
+Import ListNotations.
+
+Ltac apply_type_of__type_wf :=
+  lazymatch goal with
+  | H: type_of _ _ _ ?t |- type_wf ?t =>
+      let H' := fresh "H'" in
+      apply type_of__type_wf in H as H'
+  | H: type_of _ _ _ (TList ?t) |- type_wf ?t =>
+      let H' := fresh "H'" in
+      apply type_of__type_wf in H as H'
+  | H:  type_of _ _ _ (TOption ?t) |- type_wf ?t =>
+      let H' := fresh "H'" in
+      apply type_of__type_wf in H as H'
+  | H:  type_of _ _ _ (TDict ?t _) |- type_wf ?t =>
+      let H' := fresh "H'" in
+      apply type_of__type_wf in H as H'
+  | H:  type_of _ _ _ (TDict _ ?t) |- type_wf ?t =>
+      let H' := fresh "H'" in
+      apply type_of__type_wf in H as H'
+  | H:  type_of _ _ _ (TRecord ?tl) |- context[?tl] =>
+      let H' := fresh "H'" in
+      apply type_of__type_wf in H as H'
+  end.
+
+Ltac trans_of_eq :=
+  lazymatch goal with
+    H: interp_expr _ _ ?e = _, H': _ = interp_expr _ _ ?e |- _ =>
+      rewrite H in H'; injection H'; intros; subst end.
+
+Ltac type_of_list_entry :=
+  lazymatch goal with
+  | H1: type_of _ _ ?e _, _: interp_expr _ _ ?e = VList ?l,
+        _: In ?x ?l |- type_of_value ?x _ =>
+      eapply type_sound in H1; eauto; inversion H1; subst;
+      trans_of_eq;
+      apply_Forall_In end.
+
+Section fold_expr.
+  Context (f : expr -> expr).
+  Fixpoint fold_expr (e : expr) :=
+    f
+      match e with
+      | EVar _ | ELoc _ | EAtom _ => e
+      | EUnop o e => EUnop o (fold_expr e)
+      | EBinop o e1 e2 => EBinop o (fold_expr e1) (fold_expr e2)
+      | EIf e1 e2 e3 => EIf (fold_expr e1) (fold_expr e2) (fold_expr e3)
+      | ELet e1 x e2 => ELet (fold_expr e1) x (fold_expr e2)
+      | EFlatmap e1 x e2 => EFlatmap (fold_expr e1) x (fold_expr e2)
+      | EFold e1 e2 x y e3 => EFold (fold_expr e1) (fold_expr e2) x y (fold_expr e3)
+      | ERecord l => ERecord (List.map (fun '(s, e) => (s, fold_expr e)) l)
+      | EAccess e x => EAccess (fold_expr e) x
+      | EDict l => EDict (List.map (fun '(e1, e2) => (fold_expr e1, fold_expr e2)) l)
+      | EInsert d k v => EInsert (fold_expr d) (fold_expr k) (fold_expr v)
+      | EDelete d k => EDelete (fold_expr d) (fold_expr k)
+      | ELookup d k => ELookup (fold_expr d) (fold_expr k)
+      | EOptMatch e e_none x e_some => EOptMatch (fold_expr e) (fold_expr e_none) x (fold_expr e_some)
+      | EDictFold d e0 k v acc e => EDictFold (fold_expr d) (fold_expr e0) k v acc (fold_expr e)
+      | ESort l => ESort (fold_expr l)
+      | EFilter e x p => EFilter (fold_expr e) x (fold_expr p)
+      | EJoin e1 e2 x y p r => EJoin (fold_expr e1) (fold_expr e2) x y (fold_expr p) (fold_expr r)
+      | EProj e x r => EProj (fold_expr e) x (fold_expr r)
+      end.
+End fold_expr.
+
+Section WithMap.
+  Context {width: Z} {word: word.word width} {word_ok: word.ok word}.
+  Notation value := (value (width:=width)).
+  Context {tenv : map.map string type} {tenv_ok : map.ok tenv}.
+  Context {locals : map.map string value} {locals_ok : map.ok locals}.
+
+  Ltac apply_fold_expr_preserve_ty_IH :=
+    lazymatch goal with
+    | IH: context[type_of _ _ (fold_expr _ ?e) _] |- type_of _ _ (fold_expr _ ?e) _ =>
+        apply IH; auto
+    end.
+
+  Lemma fold_expr_preserve_ty : forall Gstore f,
+      preserve_ty Gstore f -> preserve_ty Gstore (fold_expr f).
+  Proof.
+    unfold preserve_ty. intros * H * ? ? ?.
+    generalize dependent Genv; generalize dependent t. induction e using expr_IH;
+      intros; simpl; auto;
+      apply H; invert_type_of_clear; subst; try econstructor; eauto.
+    all: try apply_fold_expr_preserve_ty_IH; repeat apply tenv_wf_step; auto;
+      try now (apply_type_of__type_wf; eauto; try invert_type_wf; auto).
+    1: apply type_of__type_wf in H10; auto.
+    4: apply type_of__type_wf in H11; auto.
+    1: rewrite fst_map_fst; auto.
+    1:{ lazymatch goal with H1: NoDup _, H2: Permutation _ _,
+            H3: List.map fst _ = _ |- _ =>
+                              clear H1 H2 H3 end.
+        generalize dependent tl. induction l; auto. intros.
+        destruct tl; invert_Forall2; try discriminate. simpl in *.
+        constructor.
+        2: apply IHl; invert_Forall; intuition auto.
+        invert_Forall. destruct a; simpl in *. apply H5; auto. }
+    1:{ induction l; simpl; auto. repeat invert_Forall. constructor.
+        2:{ apply IHl; intuition auto. }
+        destruct a; simpl in *. intuition auto. }
+  Qed.
+
+  Ltac apply_fold_expr_preserve_sem_IH :=
+    multimatch goal with
+    | IH: context[interp_expr _ _ (fold_expr _ ?e)],
+        _: type_of _ ?G ?e _ |- context[interp_expr _ _ (fold_expr _ ?e)] =>
+        erewrite IH with (Genv:=G); eauto
+    end.
+
+  Lemma fold_expr_preserve_sem : forall Gstore (store : locals) f,
+      preserve_ty Gstore f ->
+      preserve_sem Gstore store f -> preserve_sem Gstore store (fold_expr f).
+  Proof.
+    unfold preserve_sem; intros * ? H_sem. induction e using expr_IH; simpl; auto; intros.
+    1-3: erewrite H_sem; eauto.
+    all: invert_type_of_clear.
+    all: try now (erewrite H_sem; eauto;
+                  [ simpl; repeat apply_fold_expr_preserve_sem_IH
+                  | econstructor; eauto; apply fold_expr_preserve_ty ];
+                  eauto with fiat2_hints).
+    1:{ erewrite H_sem; eauto.
+        2: econstructor; eauto; apply fold_expr_preserve_ty; eauto with fiat2_hints.
+        simpl; apply_fold_expr_preserve_sem_IH. case_match; auto.
+        f_equal. apply In_flat_map_ext; intros.
+        apply_fold_expr_preserve_sem_IH; eauto with fiat2_hints.
+        apply locals_wf_step; auto; type_of_list_entry. }
+    1:{ erewrite H_sem; eauto.
+        2: econstructor; eauto; apply fold_expr_preserve_ty; eauto;
+        repeat apply tenv_wf_step; eauto with fiat2_hints.
+        simpl; apply_fold_expr_preserve_sem_IH. case_match; auto.
+        apply_fold_expr_preserve_sem_IH.
+        eapply In_fold_right_ext with (P:=fun a => type_of_value a t); intros.
+        1: eapply type_sound; eauto.
+        apply_type_sound e1; rewrite_l_to_r; invert_type_of_value.
+        apply_Forall_In; intuition;
+          [ apply_fold_expr_preserve_sem_IH | eapply type_sound; resolve_locals_wf; eauto ];
+          repeat apply tenv_wf_step; repeat apply locals_wf_step;
+          eauto with fiat2_hints.
+        apply fold_expr_preserve_ty; repeat apply tenv_wf_step; eauto with fiat2_hints. }
+    1:{ erewrite H_sem with (t:=TRecord tl'); eauto.
+        2:{ econstructor; eauto.
+            1: rewrite fst_map_fst; auto.
+            1: lazymatch goal with
+               | H1: Permutation _ _, H2: NoDup _, H3: List.map fst _ = _ |- _ =>
+                   clear H1 H2 H3
+               end. generalize dependent tl. induction l; simpl; auto; intros.
+            destruct tl; simpl in *; invert_Forall2.
+            constructor. 2: apply IHl; invert_Forall; intuition.
+            case_match; simpl in *.
+            apply fold_expr_preserve_ty; auto. }
+        simpl. do 2 f_equal.
+        lazymatch goal with
+        | H1: Permutation _ _, H2: NoDup _, H3: List.map fst _ = _ |- _ =>
+            clear H1 H2 H3
+        end. generalize dependent tl; induction l; simpl; auto; intros.
+        destruct tl; invert_Forall2.
+        invert_Forall; case_match; simpl in *.
+        f_equal. 2: eapply IHl; eauto.
+        f_equal; eauto. }
+    1:{ erewrite H_sem; eauto.
+        2:{ econstructor.
+            3:{ induction l; simpl; auto.
+                repeat invert_Forall.
+                case_match; constructor; simpl in *.
+                2: apply IHl; intuition.
+                intuition; apply fold_expr_preserve_ty; eauto. }
+            all: auto. }
+        simpl. do 3 f_equal. induction l; simpl; auto.
+        repeat invert_Forall; case_match; simpl in *.
+        f_equal. 2: apply IHl; intuition.
+        f_equal; intuition; apply_fold_expr_preserve_sem_IH. }
+    1:{ erewrite H_sem; eauto.
+        2: econstructor; eapply fold_expr_preserve_ty; eauto with fiat2_hints.
+        simpl. apply_fold_expr_preserve_sem_IH. repeat case_match; auto.
+        all: apply_fold_expr_preserve_sem_IH; eauto with fiat2_hints.
+        apply locals_wf_step; eauto. eapply type_sound in H10; eauto. inversion H10; subst.
+        all: trans_of_eq; congruence. }
+    1:{ erewrite H_sem; eauto.
+        2: econstructor; eauto; apply fold_expr_preserve_ty; eauto;
+        repeat apply tenv_wf_step; eauto with fiat2_hints.
+        simpl; apply_fold_expr_preserve_sem_IH. case_match; auto.
+        apply_fold_expr_preserve_sem_IH.
+        eapply In_fold_right_ext with (P:=fun a => type_of_value a t); intros.
+        1: eapply type_sound; eauto.
+        apply_type_sound e1; rewrite_l_to_r; invert_type_of_value.
+        apply_Forall_In; intuition;
+          [ apply_fold_expr_preserve_sem_IH | eapply type_sound; resolve_locals_wf; eauto ];
+          repeat apply tenv_wf_step; repeat apply locals_wf_step;
+          eauto with fiat2_hints.
+        apply fold_expr_preserve_ty; repeat apply tenv_wf_step; eauto with fiat2_hints. }
+    1:{ erewrite H_sem; eauto.
+        2: econstructor; eauto; apply fold_expr_preserve_ty; eauto with fiat2_hints.
+        simpl. apply_fold_expr_preserve_sem_IH. case_match; auto.
+        f_equal. apply In_filter_ext; intros.
+        apply_fold_expr_preserve_sem_IH; eauto with fiat2_hints.
+        apply locals_wf_step; auto. type_of_list_entry. }
+    1:{ erewrite H_sem; eauto.
+        2: econstructor; eauto; apply fold_expr_preserve_ty;
+        repeat apply tenv_wf_step; eauto with fiat2_hints.
+        simpl. repeat apply_fold_expr_preserve_sem_IH. repeat case_match; auto.
+        f_equal. apply In_flat_map_ext; intros. erewrite In_filter_ext.
+        1: apply map_ext_in; intros.
+        2: simpl; intros.
+        all: apply_fold_expr_preserve_sem_IH;
+          [ repeat apply tenv_wf_step | repeat apply locals_wf_step ]; eauto with fiat2_hints.
+        all: try type_of_list_entry.
+        all: lazymatch goal with H: In _ (filter _ _) |- _ => apply filter_In in H; intuition end.
+        type_of_list_entry. }
+    1:{ erewrite H_sem; eauto.
+        2: econstructor; eauto; apply fold_expr_preserve_ty; eauto with fiat2_hints.
+        simpl. apply_fold_expr_preserve_sem_IH. case_match; auto.
+        f_equal. apply map_ext_in; intros.
+        apply_fold_expr_preserve_sem_IH; eauto with fiat2_hints.
+        repeat apply locals_wf_step; auto; type_of_list_entry. }
+  Qed.
+
+  Lemma fold_expr_sound : forall f,
+      expr_transf_sound (locals:=locals) f ->
+      expr_transf_sound (locals:=locals) (fold_expr f).
+  Proof.
+    unfold expr_transf_sound; intuition idtac.
+    1:{ apply fold_expr_preserve_ty; auto.
+        unfold preserve_ty; intros; apply H; auto. }
+    1:{ eapply fold_expr_preserve_sem; resolve_locals_wf; eauto.
+        all: unfold preserve_ty, preserve_sem; intros.
+        all: apply H in H7; intuition auto. }
+  Qed.
+End WithMap.
+
+Section fold_command.
+  Context (f : command -> command).
+  Context (g : expr -> expr).
+
+  Fixpoint fold_command (c : command) : command :=
+    f
+      match c with
+      | CSkip => CSkip
+      | CSeq c1 c2 => CSeq (fold_command c1) (fold_command c2)
+      | CLet e x c => CLet (fold_expr g e) x (fold_command c)
+      | CLetMut e x c => CLetMut (fold_expr g e) x (fold_command c)
+      | CAssign x e => CAssign x (fold_expr g e)
+      | CIf e c1 c2 => CIf (fold_expr g e) (fold_command c1) (fold_command c2)
+      | CForeach e x c => CForeach (fold_expr g e) x (fold_command c)
+      end.
+End fold_command.
+
+Section WithMap.
+  Context {width: Z} {word: word.word width} {word_ok: word.ok word}.
+  Notation value := (value (width:=width)).
+  Context {tenv : map.map string type} {tenv_ok : map.ok tenv}.
+  Context {locals : map.map string value} {locals_ok : map.ok locals}.
+
+  Lemma fold_command_id_preserve_ty : forall f,
+      (forall Gstore, preserve_ty Gstore f) ->
+      forall c Gstore Genv,
+      tenv_wf Gstore -> tenv_wf Genv ->
+      well_typed Gstore Genv c -> well_typed Gstore Genv (fold_command id f c).
+  Proof.
+    induction c; simpl; auto; intros.
+    all: invert_well_typed.
+    all: econstructor; eauto with fiat2_hints;
+      try apply fold_expr_preserve_ty; auto.
+  Qed.
+
+  Ltac use_fold_command_id_preserve_sem_IH Gstore' :=
+    lazymatch goal with
+      IH: context[interp_command _ _ (fold_command id _ ?c) = _] |-
+        context[interp_command _ _ (fold_command id _ ?c)] =>
+        erewrite IH with (Gstore:=Gstore')
+    end.
+
+  Lemma fold_command_id_preserve_sem : forall f,
+      (forall Gstore, preserve_ty Gstore f) ->
+      (forall Gstore (store : locals), preserve_sem Gstore store f) ->
+      forall c (Gstore Genv : tenv) (store env : locals),
+      tenv_wf Gstore -> tenv_wf Genv ->
+      well_typed Gstore Genv c ->
+      locals_wf Gstore store -> locals_wf Genv env ->
+      interp_command store env (fold_command id f c) = interp_command store env c.
+  Proof.
+    induction c; simpl; auto; intros.
+    all: invert_well_typed.
+    1:{ repeat use_fold_command_id_preserve_sem_IH Gstore; eauto.
+        eapply command_type_sound; eauto. }
+    1:{ use_fold_command_id_preserve_sem_IH Gstore.
+        4: eauto. all: eauto with fiat2_hints.
+        2:{ apply locals_wf_step; auto. eapply type_sound with (Gstore:=Gstore); eauto.
+            apply fold_expr_preserve_ty; auto. }
+        erewrite fold_expr_preserve_sem with (Gstore:=Gstore); eauto. }
+    1:{ use_fold_command_id_preserve_sem_IH (map.put Gstore x t).
+        all: eauto with fiat2_hints.
+        2:{ apply locals_wf_step; auto. eapply type_sound with (Gstore:=Gstore); eauto.
+            apply fold_expr_preserve_ty; auto. }
+        f_equal. erewrite fold_expr_preserve_sem with (Gstore:=Gstore); eauto. }
+    1:{ f_equal. erewrite fold_expr_preserve_sem with (Gstore:=Gstore); eauto. }
+    1:{ erewrite fold_expr_preserve_sem with (Gstore:=Gstore); eauto.
+        repeat case_match; auto.
+        all: use_fold_command_id_preserve_sem_IH Gstore; eauto. }
+    1:{ erewrite fold_expr_preserve_sem with (Gstore:=Gstore); eauto.
+        repeat case_match; auto.
+        apply_type_sound e; rewrite_l_to_r.
+        invert_type_of_value.
+        repeat lazymatch goal with H: context[VList] |- _ => clear H end.
+        generalize dependent store.
+        induction l; simpl in *; auto; intros. invert_Forall.
+        rewrite IHl; auto.
+        2: eapply command_type_sound; resolve_locals_wf; eauto with fiat2_hints.
+        2: apply fold_command_id_preserve_ty; eauto with fiat2_hints.
+        f_equal. use_fold_command_id_preserve_sem_IH Gstore. 4: eauto.
+        all: eauto with fiat2_hints. }
+  Qed.
+
+  Lemma fold_command_id_sound : forall f,
+      expr_transf_sound (locals:=locals) f ->
+      transf_sound (locals:=locals) (fun _ _ => fold_command id f).
+  Proof.
+    unfold expr_transf_sound, transf_sound; intros; split.
+    1:{ apply fold_command_id_preserve_ty; auto.
+        unfold preserve_ty; intros.
+        lazymatch goal with
+          H: context[_ -> _ /\ _], H': type_of _ _ _ _ |- _ =>
+            apply H in H' end; intuition idtac. }
+    1:{ intros. erewrite fold_command_id_preserve_sem;
+        resolve_locals_wf; eauto;
+        unfold preserve_ty, preserve_sem; intros;
+        lazymatch goal with
+              H: context[_ -> _ /\ _], H': type_of _ _ _ _ |- _ =>
+                apply H in H' end; intuition auto. }
+  Qed.
+End WithMap.
+
+Section WithGlobals.
+  Context (globals : list string).
+  Context (global_types : list type) (global_types_ok : List.length globals = List.length global_types).
+  Notation tenv_wf_with_globals := (tenv_wf_with_globals globals global_types).
+
+  Section fold_command_with_globals.
+    Context (f : expr -> expr).
+
+    Fixpoint fold_command_with_globals (c : command) : command :=
+      match c with
+      | CSkip => CSkip
+      | CSeq c1 c2 => CSeq (fold_command_with_globals c1) (fold_command_with_globals c2)
+      | CLet e x c => CLet (fold_expr f e) x (fold_command_with_globals c)
+      | CLetMut e x c =>
+          (* Avoid applying the transformation if the global variable is shadowed *)
+          CLetMut (fold_expr f e) x
+            (if inb String.eqb x globals then c else fold_command_with_globals c)
+      | CAssign x e => CAssign x (fold_expr f e)
+      | CIf e c1 c2 =>
+          CIf (fold_expr f e) (fold_command_with_globals c1) (fold_command_with_globals c2)
+      | CForeach e x c =>
+          CForeach (fold_expr f e) x (fold_command_with_globals c)
+      end.
+  End fold_command_with_globals.
+
+  Section WithMap.
+    Context {width: Z} {word: word.word width} {word_ok: word.ok word}.
+    Notation value := (value (width:=width)).
+    Context {tenv : map.map string type} {tenv_ok : map.ok tenv}.
+    Context {locals : map.map string value} {locals_ok : map.ok locals}.
+
+    Ltac invert_parameterized_wf :=
+      lazymatch goal with H: parameterized_wf _ _ _ _ |- _ => inversion H; subst end.
+
+    Ltac apply_fold_command_with_globals_preserve_ty_IH :=
+      lazymatch goal with
+      | IH: context[fold_command_with_globals _ ?c] |- context[?c] =>
+          apply IH
+      end.
+
+    Lemma fold_command_with_globals_preserve_ty : forall f,
+        (forall Gstore, tenv_wf_with_globals Gstore -> preserve_ty Gstore f) ->
+        forall c Gstore Genv,
+          tenv_wf Gstore -> tenv_wf Genv -> tenv_wf_with_globals Gstore ->
+          well_typed Gstore Genv c -> well_typed Gstore Genv (fold_command_with_globals f c).
+    Proof.
+      induction c; simpl; auto; intros.
+      all: lazymatch goal with
+             H: well_typed _ _ _ |- _ => inversion H; subst
+           end.
+      1: constructor; apply_fold_command_with_globals_preserve_ty_IH; auto.
+      all: econstructor; try now (apply fold_expr_preserve_ty; eauto).
+      all: try apply_fold_command_with_globals_preserve_ty_IH; auto.
+      1,3: apply tenv_wf_step; auto.
+      1: eapply type_of__type_wf with (Gstore:=Gstore); eauto.
+      1: lazymatch goal with
+           H: type_of _ _ _ (TList ?t) |- type_wf ?t =>
+             apply type_of__type_wf in H; auto;
+             apply invert_TList_wf in H; auto
+         end.
+      1:{ case_match; auto.
+          apply_fold_command_with_globals_preserve_ty_IH; auto.
+          1: apply tenv_wf_step; auto;
+          eapply type_of__type_wf with (Gstore:=Gstore); eauto.
+          apply tenv_wf_with_globals_step; auto.
+          rewrite inb_false_iff in *. auto. }
+    Qed.
+
+    Ltac apply_fold_command_with_globals_preserve_sem_IH :=
+      lazymatch goal with
+      | IH: context[interp_command _ _ (fold_command_with_globals _ ?c)],
+          H: parameterized_wf ?Gstore' ?Genv' _ ?c |-
+          context[interp_command _ _ (fold_command_with_globals _ ?c)] =>
+          erewrite <- IH with (Gstore:=Gstore') (Genv:=Genv'); eauto
+      end.
+
+    Context (Pv : value -> Prop).
+    Notation value_wf_with_globals := (value_wf_with_globals Pv).
+
+    Lemma fold_command_with_globals_preserve_sem : forall f c,
+        (forall (Gstore : tenv), tenv_wf_with_globals Gstore ->
+                                 preserve_ty Gstore f) ->
+        (forall (Gstore : tenv) (store : locals),
+            tenv_wf_with_globals Gstore ->
+            holds_for_all_entries (value_wf_with_globals globals) store ->
+            preserve_sem Gstore store f) ->
+        forall (Gstore Genv : tenv) (store env : locals),
+          tenv_wf Gstore -> tenv_wf Genv -> tenv_wf_with_globals Gstore ->
+          parameterized_wf Gstore Genv (value_wf_with_globals globals) c ->
+          locals_wf Gstore store -> locals_wf Genv env ->
+          holds_for_all_entries (value_wf_with_globals globals) store ->
+          interp_command store env c = interp_command store env (fold_command_with_globals f c).
+    Proof.
+      induction c; simpl; intros; auto; invert_parameterized_wf.
+      3:{ erewrite <- fold_expr_preserve_sem; eauto; case_match; auto.
+          rewrite inb_false_iff in *.
+          erewrite <- IHc; auto.
+          4:{ eapply parameterized_wf_Proper.
+              5: eauto. all: eauto.
+              apply iff2_sym. apply rm_not_in_globals; auto. }
+          all: resolve_locals_wf; eauto with fiat2_hints.
+          1: apply not_In__tenv_wf_with_globals; auto.
+          1:{ eapply type_sound; resolve_locals_wf; auto.
+              apply fold_expr_preserve_ty; eauto with fiat2_hints. }
+          unfold holds_for_all_entries.
+          1: apply not_In__value_wf_with_globals; auto. }
+      all: try erewrite <- fold_expr_preserve_sem; eauto;
+        repeat case_match; auto;
+        repeat apply_fold_command_with_globals_preserve_sem_IH; eauto with fiat2_hints.
+      1:{ eapply command_type_sound; eauto.
+          eapply parameterized_wf__well_typed; eauto. }
+      1:{ eapply parameterized_wf__preserve_P with (Gstore:=Gstore); eauto. }
+      1:{ resolve_locals_wf. erewrite fold_expr_preserve_sem; eauto with fiat2_hints. }
+      1:{ apply_type_sound e. rewrite fold_expr_preserve_sem in E; eauto. rewrite E in *.
+          lazymatch goal with H: type_of_value _ _ |- _ => inversion H; subst end.
+          lazymatch goal with
+            H1: type_of_value _ _, H2: interp_expr _ _ _ = VList _ |- _ =>
+              clear H1 H2
+          end.
+          generalize dependent store. induction l; simpl; auto; intros.
+          invert_Forall. eapply IHc in H12 as IHc'; eauto with fiat2_hints.
+          rewrite <- IHc'. apply IHl; auto.
+          2: eapply parameterized_wf__preserve_P with (Gstore:=Gstore) (Genv:=map.put Genv x t);
+          eauto with fiat2_hints.
+          apply command_type_sound with (Genv:=map.put Genv x t); auto.
+          2:{ apply tenv_wf_step; auto. apply_type_of__type_wf; auto. invert_type_wf; auto. }
+          2: eapply locals_wf_step; eauto.
+          eapply parameterized_wf__well_typed; eauto. }
+    Qed.
+
+    Ltac apply_preserve_parameterized_wf_IH :=
+      lazymatch goal with
+        IH: context[fold_command_with_globals _ ?c] |- context[?c] =>
+          apply IH
+      end.
+
+    Lemma fold_command_with_globals_preserve_index_wf : forall f,
+        (forall (Gstore : tenv), tenv_wf_with_globals Gstore ->
+                                 preserve_ty Gstore f) ->
+        (forall (Gstore : tenv) (store : locals),
+            tenv_wf_with_globals Gstore ->
+            holds_for_all_entries (value_wf_with_globals globals) store ->
+            preserve_sem Gstore store f) ->
+        forall c (Gstore Genv : tenv),
+          tenv_wf Gstore -> tenv_wf Genv ->
+          tenv_wf_with_globals Gstore ->
+          parameterized_wf Gstore Genv (value_wf_with_globals globals) c ->
+          parameterized_wf Gstore Genv (value_wf_with_globals globals) (fold_command_with_globals f c).
+    Proof.
+      induction c; simpl; auto; intros; invert_parameterized_wf.
+      all: try (econstructor;
+                try (apply fold_expr_preserve_ty; eauto);
+                apply_preserve_parameterized_wf_IH; eauto with fiat2_hints).
+      1:{ econstructor.
+          1: apply fold_expr_preserve_ty; eauto.
+          case_match; auto. rewrite inb_false_iff in *.
+          eapply parameterized_wf_Proper.
+          4: apply rm_not_in_globals.
+          all: eauto. apply_preserve_parameterized_wf_IH; eauto with fiat2_hints.
+          1: apply tenv_wf_with_globals_step; auto.
+          eapply parameterized_wf_Proper.
+          4: apply iff2_sym, rm_not_in_globals.
+          all: eauto. }
+      1:{ econstructor; eauto.
+          2: apply fold_expr_preserve_ty; eauto.
+          intros. erewrite fold_expr_preserve_sem; eauto. }
+    Qed.
+  End WithMap.
+End WithGlobals.
+
+
+Section WithMap.
+  Context {width: Z} {word: word.word width} {word_ok: word.ok word}.
+  Notation value := (value (width:=width)).
+  Context {tenv : map.map string type} {tenv_ok : map.ok tenv}.
+  Context {locals : map.map string value} {locals_ok : map.ok locals}.
+
+  Section WithIndex.
+    Context {consistency : Type} (consistent : consistency -> value -> value -> Prop).
+    Context {to_from_con from_to_con : consistency}.
+    Context {idx : IndexInterface.index} {idx_wf : value -> Prop} {idx_ok : ok to_from_con from_to_con idx idx_wf consistent}.
+
+    Notation expr_aug_transf_sound := (expr_aug_transf_sound (idx_wf:=idx_wf)).
+    Notation aug_transf_sound := (aug_transf_sound (idx_wf:=idx_wf)).
+
+    Lemma fold_command_with_globals_sound : forall f,
+        expr_aug_transf_sound f ->
+        aug_transf_sound (fun x => fold_command_with_globals [x] (f x)).
+    Proof.
+      unfold expr_aug_transf_sound, aug_transf_sound; intros; intuition idtac.
+      3: symmetry; eapply fold_command_with_globals_preserve_sem;
+      resolve_locals_wf; eauto; auto.
+      2: eapply fold_command_with_globals_preserve_index_wf; eauto; auto.
+      1: eapply fold_command_with_globals_preserve_ty; eauto; try reflexivity.
+      all: try (unfold preserve_ty; intros; eapply H; eauto).
+      all: unfold preserve_sem; intros;
+        lazymatch goal with
+          H: context[type_of _ _ _ _ -> _], H': type_of _ _ _ _ |- _ =>
+            eapply H in H' as [HL HR]; eauto end; erewrite HR; eauto.
+    Qed.
+  End WithIndex.
+End WithMap.
+
+Section fold_command_with_global.
+  (* Useful for whole-program to-index transformation *)
+  Context (tbl : string).
+  Context (f : list string -> command -> command).
+  Context (g : expr -> expr).
+  Fixpoint fold_command_with_global (free_vars : list string) (c : command) : command :=
+    f free_vars
+      match c with
+      | CSkip => CSkip
+      | CSeq c1 c2 => CSeq (fold_command_with_global free_vars c1) (fold_command_with_global free_vars c2)
+      | CLet e x c => CLet (fold_expr g e) x (fold_command_with_global (x :: free_vars) c)
+      | CLetMut e x c =>
+          (* Avoid applying the transformation if the global variable is shadowed *)
+          CLetMut (fold_expr g e) x
+            (if String.eqb x tbl then c else fold_command_with_global free_vars c)
+      | CAssign x e => CAssign x (fold_expr g e)
+      | CIf e c1 c2 =>
+          CIf (fold_expr g e) (fold_command_with_global free_vars c1) (fold_command_with_global free_vars c2)
+      | CForeach e x c =>
+          CForeach (fold_expr g e) x (fold_command_with_global (x :: free_vars) c)
+      end.
+End fold_command_with_global.
+
+#[export] Hint Resolve fold_command_with_globals_sound : transf_hints.
+#[export] Hint Resolve fold_command_id_sound : transf_hints.
+
+
+Section WithMap.
+  Context {width: Z} {word: word.word width} {word_ok: word.ok word}.
+  Notation value := (value (width:=width)).
+  Context {tenv : map.map string type} {tenv_ok : map.ok tenv}.
+  Context {locals : map.map string value} {locals_ok : map.ok locals}.
+
+  Definition singleton_rel x (y y' : string) :=
+    y = x /\ y' = x.
+
+  Lemma singleton_rel_refl : forall (s : string),
+      singleton_rel s s s.
+  Proof.
+    unfold singleton_rel; intuition auto.
+  Qed.
+
+  Definition sem_eq (Gstore Genv : tenv) (t : type) (e1 e2 : expr) :=
+    type_of Gstore Genv e1 t /\ type_of Gstore Genv e2 t /\
+      forall (store env : locals),
+        locals_wf Gstore store -> locals_wf Genv env ->
+        interp_expr store env e1 = interp_expr store env e2.
+
+  Lemma sem_eq_sym  (Gstore Genv : tenv) (t : type) : forall e1 e2,
+      sem_eq Gstore Genv t e1 e2 -> sem_eq Gstore Genv t e2 e1.
+  Proof.
+    unfold sem_eq; intros. intuition auto. symmetry. auto.
+  Qed.
+
+  Lemma sem_eq_trans  (Gstore Genv : tenv) (t : type) : forall e1 e2 e3,
+      sem_eq Gstore Genv t e1 e2 ->
+      sem_eq Gstore Genv t e2 e3 ->
+      sem_eq Gstore Genv t e1 e3.
+  Proof.
+    unfold sem_eq; intros. intuition auto.
+    rewrite H4, H5; auto.
+  Qed.
+
+  Instance EFilter_Proper {t : type} (x0 : string) (Gstore Genv : tenv) :
+    tenv_wf Gstore -> tenv_wf Genv ->
+    Proper (sem_eq Gstore Genv (TList t) ==> singleton_rel x0 ==> sem_eq Gstore (map.put Genv x0 t) TBool ==> sem_eq Gstore Genv (TList t)) EFilter.
+  Proof.
+    intros * ? ? e1 e1' H1 y y' Hy e2 e2' H2.
+    unfold sem_eq in *; intros.
+    unfold singleton_rel in *. intuition auto; subst.
+    1,2: constructor; auto.
+    repeat invert_type_of.
+    simpl. lazymatch goal with
+      H: context[interp_expr _ _ ?e = _] |-
+        context[match interp_expr _ _ ?e with _ => _ end] =>
+        rewrite H end; auto.
+    case_match; auto. f_equal.
+    apply filter_ext_in; intros.
+    lazymatch goal with
+      H: context[interp_expr _ _ ?e = _] |-
+        context[match interp_expr _ _ ?e with _ => _ end] =>
+        rewrite H end; eauto with fiat2_hints.
+    apply_type_sound e1'; auto. rewrite_l_to_r.
+    apply locals_wf_step; auto. do_injection2; subst.
+    invert_type_of_value. apply_Forall_In.
+  Qed.
+
+  Lemma sem_eq_eq : forall Gstore Genv t e1 e2,
+      sem_eq Gstore Genv t e1 e2 ->
+      forall store env : locals,
+        locals_wf Gstore store -> locals_wf Genv env ->
+        interp_expr store env e1 = interp_expr store env e2.
+  Proof.
+    unfold sem_eq; intros; intuition auto.
+  Qed.
+
+  Lemma sem_eq_refl : forall Gstore Genv t e, type_of Gstore Genv e t -> sem_eq Gstore Genv t e e.
+  Proof.
+    unfold sem_eq; intuition auto.
+  Qed.
+End WithMap.
